src/Init/Grind/grindresugartests.lean
@@ -1,0 +1,2 @@
+theorem mythm (f : Nat → Nat) (h : a = b) : f (f b) = f (f a) := by
+  grind
